revm: execute test for static_call

RocqOfRust/alloy_primitives/bits/simulate/fixed.v
@@ -1,12 +1,36 @@
 Require Import simulate.RocqOfRust.
 Require Export alloy_primitives.bits.links.fixed.
 Require Import alloy_primitives.links.aliases.
+Require Import core.links.array.
+
+Module FixedBytes.
+  (** Convert to [Z] interpreting in big-endian. *)
+  Definition to_Z {N : usize} (x : FixedBytes.t N) : Z :=
+    let bytes := ArrayPairs.to_list x.(FixedBytes.value).(array.value) in
+    List.fold_left (fun acc byte => 256 * acc + i[byte] : Z) bytes 0.
+
+  (** Generate n bytes in big-endian order directly as ArrayPairs. *)
+  Fixpoint bytes_be (n : nat) (value : Z) : ArrayPairs.t u8 n :=
+    match n return ArrayPairs.t u8 n with
+    | O => ArrayEmpty.Make
+    | S n' =>
+      let shift := (Z.of_nat n' * 8)%Z in
+      {| ArrayPair.x := {| Integer.value := (value / 2 ^ shift) mod 256 |};
+         ArrayPair.xs := bytes_be n' value |}
+    end.
+
+  (** Convert from [Z] interpreting in big-endian. *)
+  Definition from_Z {N : usize} (value : Z) : FixedBytes.t N :=
+    let n := Z.to_nat N.(Integer.value) in
+    {| FixedBytes.value := {| array.value := bytes_be n value |} |}.
+End FixedBytes.
 
 Module Impl_From_U256_for_FixedBytes_32.
   Definition Self : Set :=
     FixedBytes.t {| Integer.value := 32 |}.
 
-  Parameter from : aliases.U256.t -> Self.
+  Definition from (value : aliases.U256.t) : Self :=
+    FixedBytes.from_Z value.(lib.Uint.value).
 
   Lemma from_eq (value : aliases.U256.t) (stack : Stack.t) :
     {{
