RocqOfRust/alloy_primitives/bits/simulate/address.v
@@ -1,12 +1,14 @@
 Require Import simulate.RocqOfRust.
 Require Import alloy_primitives.bits.links.address.
 Require Import alloy_primitives.bits.links.fixed.
+Require Import alloy_primitives.bits.simulate.fixed.
 
 Module Impl_Address.
   Definition Self : Set :=
     Address.t.
 
-  Parameter from_word : FixedBytes.t {| Integer.value := 32 |} -> Self.
+  Definition from_word (value : FixedBytes.t {| Integer.value := 32 |}) : Self :=
+    {| Address.value := FixedBytes.to_Z value mod (2^160) |}.
 
   Lemma from_word_eq (value : FixedBytes.t {| Integer.value := 32 |}) (stack : Stack.t) :
     {{
